src/Init/Data/Iterators/Combinators/Monadic/Sigma.lean
@@ -1,0 +1,145 @@
+/-
+Copyright (c) 2025 Lean FRO, LLC. All rights reserved.
+Released under Apache 2.0 license as described in the file LICENSE.
+Authors: Paul Reichert
+-/
+module
+
+prelude
+public import Init.Data.Iterators.Internal.Termination
+public import Init.Data.Iterators.Consumers.Loop
+
+public section
+
+namespace Std.Iterators.Types
+
+/--
+Internal state of the `sigma` combinator. Do not depend on its internals.
+-/
+@[unbox]
+structure SigmaIterator (γ : Type w) (α : γ → Type w) where
+  parameter : γ
+  inner : α parameter
+
+@[always_inline, inline]
+def SigmaIterator.Monadic.modifyStep {β γ : Type w} {α : γ → Type w} {m : Type w → Type w'}
+    [∀ x : γ, Iterator (α := α x) m β]
+    (it : IterM (α := SigmaIterator γ α) m β)
+    (step : (toIterM it.internalState.inner m β).Step) :
+    IterStep (IterM (α := SigmaIterator γ α) m β) β :=
+  match step.val with
+  | .yield it' out =>
+    .yield ⟨it.internalState.parameter, it'.internalState⟩ out
+  | .skip it' =>
+    .skip ⟨it.internalState.parameter, it'.internalState⟩
+  | .done => .done
+
+instance SigmaIterator.instIterator {γ : Type w} {α : γ → Type w}
+    [∀ x : γ, Iterator (α := α x) m β] [Monad m] :
+    Iterator (SigmaIterator γ α) m β where
+  IsPlausibleStep it step := ∃ step', Monadic.modifyStep it step' = step
+  step it :=
+    (fun step => .deflate ⟨Monadic.modifyStep it step.inflate, step.inflate, rfl⟩) <$>
+      (toIterM it.internalState.inner m β).step
+
+private structure SigmaIteratorWF (γ : Type w) (α : γ → Type w) (m : Type w → Type w) (β : Type w) where
+  parameter : γ
+  it : IterM (α := α parameter) m β
+
+private def SigmaIterator.instFinitenessRelation {γ : Type w} {α : γ → Type w}
+    [∀ x : γ, Iterator (α x) m β] [∀ x : γ, Finite (α x) m] [Monad m] :
+    FinitenessRelation (SigmaIterator γ α) m where
+  rel := InvImage
+    (PSigma.Lex emptyRelation
+      (β := fun param : γ => IterM (α := α param) m β)
+      (fun _ => InvImage IterM.TerminationMeasures.Finite.Rel IterM.finitelyManySteps))
+    (fun it => ⟨it.internalState.parameter, toIterM it.internalState.inner m β⟩)
+  wf := by
+    apply InvImage.wf
+    refine ⟨fun ⟨param, it⟩ => ?_⟩
+    apply PSigma.lexAccessible
+    · exact emptyWf.wf.apply param
+    · exact fun param' => InvImage.wf _ WellFoundedRelation.wf
+  subrelation {it it'} h := by
+    obtain ⟨_, hs, step, h', rfl⟩ := h
+    cases step using PlausibleIterStep.casesOn
+    · cases hs
+      apply PSigma.Lex.right
+      exact IterM.TerminationMeasures.Finite.rel_of_yield ‹_›
+    · cases hs
+      apply PSigma.Lex.right
+      exact IterM.TerminationMeasures.Finite.rel_of_skip ‹_›
+    · cases hs
+
+instance SigmaIterator.instFinite {γ : Type w} {α : γ → Type w}
+    [∀ x : γ, Iterator (α x) m β] [∀ x : γ, Finite (α x) m] [Monad m] :
+    Finite (SigmaIterator γ α) m :=
+  .of_finitenessRelation instFinitenessRelation
+
+private def SigmaIterator.instProductivenessRelation {γ : Type w} {α : γ → Type w}
+    [∀ x : γ, Iterator (α x) m β] [∀ x : γ, Productive (α x) m] [Monad m] :
+    ProductivenessRelation (SigmaIterator γ α) m where
+  rel := InvImage
+    (PSigma.Lex emptyRelation
+      (β := fun param : γ => IterM (α := α param) m β)
+      (fun _ => InvImage IterM.TerminationMeasures.Productive.Rel IterM.finitelyManySkips))
+    (fun it => ⟨it.internalState.parameter, toIterM it.internalState.inner m β⟩)
+  wf := by
+    apply InvImage.wf
+    refine ⟨fun ⟨param, it⟩ => ?_⟩
+    apply PSigma.lexAccessible
+    · exact emptyWf.wf.apply param
+    · exact fun param' => InvImage.wf _ WellFoundedRelation.wf
+  subrelation {it it'} h := by
+    obtain ⟨step, hs⟩ := h
+    cases step using PlausibleIterStep.casesOn
+    · cases hs
+    · cases hs
+      apply PSigma.Lex.right
+      exact IterM.TerminationMeasures.Productive.rel_of_skip ‹_›
+    · cases hs
+
+instance SigmaIterator.instProductive {γ : Type w} {α : γ → Type w}
+    [∀ x : γ, Iterator (α x) m β] [∀ x : γ, Productive (α x) m] [Monad m] :
+    Productive (SigmaIterator γ α) m :=
+  .of_productivenessRelation instProductivenessRelation
+
+instance SigmaIterator.instIteratorCollect {γ : Type w} {α : γ → Type w}
+    [∀ x : γ, Iterator (α x) m β] [Monad m] [Monad n] :
+    IteratorCollect (SigmaIterator γ α) m n :=
+  .defaultImplementation
+
+instance SigmaIterator.instIteratorCollectPartial {γ : Type w} {α : γ → Type w}
+    [∀ x : γ, Iterator (α x) m β] [Monad m] [Monad n] :
+    IteratorCollectPartial (SigmaIterator γ α) m n :=
+  .defaultImplementation
+
+instance SigmaIterator.instIteratorLoop {γ : Type w} {α : γ → Type w}
+    [∀ x : γ, Iterator (α x) m β] [Monad m] [Monad n] :
+    IteratorLoop (SigmaIterator γ α) m n :=
+  .defaultImplementation
+
+instance SigmaIterator.instIteratorLoopPartial {γ : Type w} {α : γ → Type w}
+    [∀ x : γ, Iterator (α x) m β] [Monad m] [Monad n] :
+    IteratorLoopPartial (SigmaIterator γ α) m n :=
+  .defaultImplementation
+
+end Types
+
+/--
+If the state `α param` of an iterator `it` is dependent on some parameter `param`, creates an iterator
+whose state is equivalent to the `Sigma` type `(param : γ) × α param`, getting rid of the type
+dependency at the cost of storing the parameter in a structure field at runtime.
+
+**Termination properties:**
+
+* `Finite` instance: only if the base iterator is finite
+* `Productive` instance: only if the base iterator is productive
+-/
+@[always_inline, inline, expose]
+def IterM.sigma {γ : Type w} {α : γ → Type w}
+    [∀ x : γ, Iterator (α x) m β] {param : γ} (it : IterM (α := α param) m β) :
+    IterM (α := Types.SigmaIterator γ α) m β :=
+  toIterM ⟨param, it.internalState⟩ m β
+
+end Std.Iterators
