src/Init/Data/Iterators/Combinators/Sigma.lean
@@ -1,0 +1,22 @@
+/-
+Copyright (c) 2025 Lean FRO, LLC. All rights reserved.
+Released under Apache 2.0 license as described in the file LICENSE.
+Authors: Paul Reichert
+-/
+module
+
+prelude
+public import Init.Data.Iterators.Combinators.Monadic.Sigma
+public import Init.Data.Iterators.Combinators.FilterMap
+
+public section
+
+namespace Std.Iterators
+
+@[always_inline, inline, expose, inherit_doc IterM.sigma]
+def Iter.sigma {γ : Type w} {α : γ → Type w}
+    [∀ x : γ, Iterator (α x) Id β] {param : γ} (it : Iter (α := α param) β):
+    Iter (α := Types.SigmaIterator γ α) β :=
+  it.toIterM.sigma.toIter
+
+end Std.Iterators
